theories/product.v
@@ -600,12 +600,12 @@ Lemma mod_map_step_i {EV1 EV2 S} m (f : mod_map_fn EV1 EV2 S) σ σf P `{!TStepI
 Proof.
   constructor => G /tstepi_proof HP.
   apply: (steps_impl_submodule _ (mod_map _ _) (λ x, (x, σf))); [done| |].
-  - move => ?? /= [?[HG HG']]. eexists _. split; [by apply HG|] => ? /= /HG'[?[??]]. naive_solver.
+  - move => ?? /= [?[?[HG [? HG']]]]. eexists _, _. split_and!; [by apply HG|done|] => ? /= /HG'[?[??]]. naive_solver.
   - move => ????. invert_all' @m_step; simplify_eq/=; eexists _, _.
     all: split_and!; [done| |repeat case_match => //;naive_solver].
-    + move => [?[HG HG']]. case_match; simplify_eq.
-      eexists _. split; [by apply HG|] => ? /= /HG'[?[??]]. naive_solver.
-    + move => [?[HG HG']]. eexists _. split; [by apply HG|] => ? /= /HG'[?[??]]. naive_solver.
+    + move => [?[?[HG [? HG']]]]. case_match; simplify_eq.
+      eexists _, _. split_and!; [by apply HG|done|] => ? /= /HG'[?[??]]. naive_solver.
+    + move => [?[?[HG [? HG']]]]. eexists _,_. split_and!; [by apply HG|done|] => ? /= /HG'[?[??]]. naive_solver.
 Qed.
 Global Hint Resolve mod_map_step_i : tstep.
 
